Automated commit:     This is a snapshot of the theories as present in coqfinitgroup trunk revision 1989, prepared for trunk and v8.3     This commit has been tested at commit time to work with  GNU Make 3.81.     and Ocaml 3.11.1.     under Coq trunk SVN r12934 for the trunk version     and Coq v8.3 SVN r12935 for the v8.3 version
git-svn-id: svn+ssh://scm.gforge.inria.fr/svnroot/coqfinitgroup/trunk@1994 305884b8-be16-0410-aa53-a3be2363cef1

ssreflect/ssreflect12_trunk/theories/orderedalg.v
@@ -223,7 +223,7 @@ Lemma ltrWN : forall x y, x < y -> x == y = false.
 Proof. by move=> x y; rewrite ltr_neqAle; case/andP; move/negPf=> ->. Qed.
 Hint Resolve ltrWN.
 
-Definition ltrE x y (hxy : x < y) := (hxy,(ltrWN hxy),(ltrW hxy)).
+Definition ltrE x y (hxy : x < y) := (hxy, (ltrWN hxy), (ltrW hxy)).
 
 Lemma ler_lt_trans : forall y x z, x <= y -> y < z -> x < z.
 Proof. move=> y x z lxy; apply: contra=> lzx; exact: ler_trans lxy. Qed.
@@ -247,7 +247,7 @@ CoInductive le_xor_gtr (x y : R) : bool -> bool -> Set :=
   | GtrNotLe of y < x  : le_xor_gtr x y false true.
 
 Lemma lerP : forall x y, le_xor_gtr x y (x <= y) (y < x).
-Proof. by move=> x y; case hxy: (_<=_); constructor; rewrite ?hxy //. Qed.
+Proof. by move=> x y; case hxy: (_ <= _); constructor; rewrite ?hxy //. Qed.
 
 CoInductive ltr_xor_geq (x y : R) : bool -> bool -> Set :=
   | LtrNotGeq of x < y  : ltr_xor_geq x y false true
@@ -316,6 +316,42 @@ Proof. by move=> z x y; rewrite ler_addrA addrC opprK. Qed.
 Definition ler_subr z x y := (esym (ler_addrA z x y), ler_subrA z x y).
 Definition ler_subl z x y := (esym (ler_addlA z x y), ler_sublA z x y).
 
+Lemma ler_addpl : forall x y z, 0 <= x -> y <= z -> y <= x + z.
+Proof. move=> x y z h1 h2; rewrite -(add0r y); exact: ler_add. Qed.
+
+Lemma ler_addpr : forall x y z, 0 <= z -> x <= y -> x <= y + z.
+Proof. move=> x y z h1 h2; rewrite -(addr0 x); exact: ler_add. Qed.
+
+Lemma ltr_addspl : forall x y z, 0 < x -> y < z -> y < x + z.
+Proof. move=> x y z h1 h2; rewrite -(add0r y); exact: ltr_add. Qed.
+
+Lemma ltr_addspr : forall x y z, 0 < z -> x < y -> x < y + z.
+Proof. move=> x y z h1 h2; rewrite -(addr0 x); exact: ltr_add. Qed.
+
+
+Lemma ler_addrr : forall x y,  (y <= y + x) = (0 <= x).
+Proof. by move=> x y; rewrite -{1}(addr0 y) ler_add2r. Qed.
+
+Lemma ler_addrl : forall x y, (y <= x + y) = (0 <= x).
+Proof. by move=> x y; rewrite addrC ler_addrr. Qed.
+
+Lemma ler_addll : forall x y, (x + y <= y) = (x <= 0).
+Proof. by move=> x y; rewrite -{2}(add0r y) ler_add2l. Qed.
+
+Lemma ler_addlr : forall x y, (y + x <= y) = (x <= 0).
+Proof. by move=> x y; rewrite addrC ler_addll. Qed.
+
+Lemma ltr_le_addpl : forall x y z, 0 < x -> y <= z -> y < x + z.
+Proof. by move=> x y z h1 h2; rewrite (@ler_lt_trans z) // ler_addll. Qed.
+
+Lemma ltr_le_addpr : forall x y z, 0 < x -> y <= z -> y < z + x.
+Proof. by move=> x y z h1 h2; rewrite addrC ltr_le_addpl. Qed.
+
+Lemma ltr_addpr : forall x y z, 0 <= x -> y < z -> y < x + z.
+Proof. by move=> x y z h1 h2; rewrite (@ltr_le_trans z) // ler_addrl. Qed.
+
+Lemma ltr_addpl : forall x y z, 0 <= x -> y < z -> y < z + x.
+Proof. by move=> x y z h1 h2; rewrite addrC ltr_addpr. Qed.
 
 Lemma ler_mulpr : forall z x y, 0 <= z -> (x <= y) -> (x * z <= y * z).
 Proof.
@@ -448,13 +484,14 @@ move=> s x; case: (inF3P s)=> ->; rewrite ?(signr0,mul0r,mul1r) //.
 by rewrite signr_opp mulN1r.
 Qed.
 
-Lemma signr_exp : forall s x n, (s ?* x)^+n.+1 = (s ^+ n.+1) ?* (x ^+ n.+1).
+Lemma smul_exp : forall s x n, (s ?* x)^+n.+1 = (s ^+ n.+1) ?* (x ^+ n.+1).
 Proof.
 move=> s x n; case: (inF3P s)=> ->; first by rewrite ![0^+_.+1]exprS !mul0r.
   by rewrite exp1rn.
 rewrite [_^+_]exprN -![(-1)^+n.+1]signr_odd.
 by case: (odd n.+1); rewrite !(expr0,expr1) !(mulNr,mul1r).
 Qed.
+
 
 (* absr section *)
 Definition absr x := (\s x) ?* x.
@@ -909,7 +946,7 @@ move=> x n; case: (ltrgtP x 0)=> hx; last first.
   by rewrite absr0 exprS mul0r absr0.
 - by rewrite !ger0_abs// ltrE// expf_gt0.
 - case: n=> [|n]; first by rewrite !expr0 ger0_abs// ler01.
-  rewrite {1}[x]smul_abs_id signr_exp absr_smul.
+  rewrite {1}[x]smul_abs_id smul_exp absr_smul.
     by rewrite ger0_abs// expf_ge0// absrE.
   by rewrite (ltr0_sign hx) -signr_odd; case: (odd _).
 Qed.
@@ -1095,6 +1132,13 @@ move=> x n; rewrite -mulr_natr signr_mul -{2}[\s _]mulr1.
 by congr (_*_); apply/eqP; rewrite signr_cp0 gtf0Sn.
 Qed.
 
+
+Lemma signr_exp : forall x n, \s (x^+n) = (\s x)^+n.
+Proof.
+move=> x; elim=> [|n ihn]; first by rewrite expr0 signr1.
+by rewrite !exprSr signr_mul ihn mulrC.
+Qed.
+
 Lemma midf_le : forall x y, x <= y -> x <= (x+y)/2%:R <= y.
 Proof.
 move=> x y lxy; rewrite ?lef_divp ?gtf0Sn//.
@@ -1226,6 +1270,18 @@ Definition ler_subrA := ler_subrA.
 Definition ler_sublA := ler_sublA. 
 Definition ler_subr := ler_subr.
 Definition ler_subl := ler_subl.
+Definition ler_addpl := ler_addpl.
+Definition ler_addpr := ler_addpr.
+Definition ltr_addspl := ltr_addspl.
+Definition ltr_addspr := ltr_addspr.
+Definition ler_addrr := ler_addrr.
+Definition ler_addrl := ler_addrl.
+Definition ler_addll := ler_addll.
+Definition ler_addlr := ler_addlr.
+Definition ltr_le_addpl := ltr_le_addpl.
+Definition ltr_le_addpr := ltr_le_addpr.
+Definition ltr_addpr := ltr_addpr.
+Definition ltr_addpl := ltr_addpl.
 Definition ler_mulpr := ler_mulpr. 
 Definition ler_mulpl := ler_mulpl. 
 Definition ler_mulnr := ler_mulnr. 
@@ -1324,12 +1380,13 @@ Definition expf_ge0 := expf_ge0.
 Definition lef_expSr := lef_expSr. 
 Definition lef_exprS := lef_exprS. 
 Definition lef_expS2 := lef_expS2. 
-Definition signr_exp := signr_exp. 
+Definition smul_exp := smul_exp. 
 Definition absf_exp := absf_exp. 
 
 (* Field Theory *)
 Definition signr_mul := signr_mul.
 Definition signr_mulrn := signr_mulrn.
+Definition signr_exp := signr_exp.
 Definition mulf_ge0 := mulf_ge0.
 Definition mulf_le0 := mulf_le0.
 Definition mulf_gt0 := mulf_gt0.
